theories/rust_typing/enum/deinit.v
@@ -1,0 +1,19 @@
+From refinedrust Require Export type ltypes.
+From refinedrust Require Import uninit int int_rules.
+From refinedrust Require Import programs ltypes.
+From refinedrust Require Import options.
+
+Section rules.
+  Context `{!typeGS Σ}.
+
+  Lemma owned_subltype_step_enum_uninit π E L l {rt rte} (en : enum rt) (lte : ltype rte) rs tag re st T  :
+    owned_subltype_step π E L l #rs #() (EnumLtype en tag lte re) (◁ uninit st) T :-
+    ∀ le,
+      (*ste ← tactic (compute_map_lookup_goal (list_to_map (en.(enum_els).(els_variants))) tag false);*)
+      return owned_subltype_step π E L le #re #() lte (◁ uninit (ltype_st lte)) T.
+  Proof.
+  Admitted.
+  Definition owned_subltype_step_enum_uninit_inst := [instance owned_subltype_step_enum_uninit].
+  Global Existing Instance owned_subltype_step_enum_uninit_inst | 20.
+
+End rules.
