theories/rust_typing/enum/enum.v
@@ -1,2 +1,2 @@
 From refinedrust Require Export type ltypes.
-From refinedrust.enum Require Export def place subtype subltype unfold discriminant init.
+From refinedrust.enum Require Export def place subtype subltype unfold discriminant init deinit.
