theories/rust_typing/mut_ref/deinit.v
@@ -1,0 +1,229 @@
+From refinedrust Require Export base type ltypes.
+From refinedrust Require Import ltype_rules.
+From refinedrust Require Import programs.
+From refinedrust.mut_ref Require Import def.
+From refinedrust Require Import options.
+
+(** ** Lemmas about deinitializing *)
+
+Section deinit.
+  Context `{!typeGS Σ}.
+
+  (* TODO seem to be redundant. Rather use the stronger extractable stuff *)
+  Lemma ltype_uniq_deinitializable_deinit_mut F π l st {rt} (lt : ltype rt) r κ γ wl :
+    lftE ⊆ F →
+    ltype_uniq_deinitializable lt →
+    syn_type_compat PtrSynType st →
+    (l ◁ₗ[π, Owned wl] #(r, γ) @ (MutLtype lt κ)) ={F}=∗
+    l ◁ₗ[π, Owned false] #() @ (◁ uninit st) ∗ place_rfn_interp_mut r γ.
+  Proof.
+    iIntros (? Hdeinit Hcompat).
+    iIntros "Hl".
+    rewrite ltype_own_mut_ref_unfold /mut_ltype_own.
+    iDestruct "Hl" as "(%ly & %Halg & %Hly & Hlb & Hcred & %γ' & %r' & %Heq & Hb)".
+    injection Heq as <- <-.
+    iMod (maybe_use_credit with "Hcred Hb") as "(Hcred & Hat & Hc)"; first done.
+    iDestruct "Hc" as "(%l' & Hl & Hb)".
+    iMod (ltype_own_deinit_ghost_drop_uniq with "Hb") as "Hrfn"; [done.. | ].
+    iFrame.
+    rewrite ltype_own_ofty_unfold /lty_of_ty_own. iExists ly.
+    iSplitR. { destruct Hcompat as [<- | (ly1 & Hst' & ->)]; first done.
+      simpl. iPureIntro. eapply syn_type_has_layout_make_untyped; last done.
+      by eapply syn_type_has_layout_inj. }
+    iR. iSplitR. { rewrite /ty_own_val/=//. }
+    iSplitL "Hlb"; first by iFrame. iR.
+    iExists tt. iR. iModIntro. iExists _. iFrame.
+    rewrite uninit_own_spec. iExists ly.
+    apply syn_type_has_layout_ptr_inv in Halg as ->. iSplitR; last done.
+    iPureIntro. destruct Hcompat as [<- | (ly1 & Hst' & ->)]; first done.
+    specialize (syn_type_has_layout_ptr_inv _ Hst') as ->.
+    eapply syn_type_has_layout_make_untyped; done.
+  Qed.
+
+  (* TODO try to find a good way to unify with previous lemma *)
+  Lemma ltype_uniq_deinitializable_deinit_mut' F π l st {rt} (lt : ltype rt) r κ γ wl :
+    lftE ⊆ F →
+    ltype_uniq_deinitializable lt →
+    syn_type_compat PtrSynType st →
+    £ (Nat.b2n wl) -∗
+    (l ◁ₗ[π, Owned wl] #(r, γ) @ (MutLtype lt κ)) ={F}=∗
+    l ◁ₗ[π, Owned wl] #() @ (◁ uninit st) ∗ place_rfn_interp_mut r γ.
+  Proof.
+    iIntros (? Hdeinit Hcompat).
+    iIntros "Hcred' Hl".
+    rewrite ltype_own_mut_ref_unfold /mut_ltype_own.
+    iDestruct "Hl" as "(%ly & %Halg & %Hly & Hlb & Hcred & %γ' & %r' & %Heq & Hb)".
+    injection Heq as <- <-.
+    iMod (maybe_use_credit with "Hcred Hb") as "(Hcred & Hat & Hc)"; first done.
+    iDestruct "Hc" as "(%l' & Hl & Hb)".
+    iMod (ltype_own_deinit_ghost_drop_uniq with "Hb") as "Hrfn"; [done.. | ].
+    iFrame.
+    rewrite ltype_own_ofty_unfold /lty_of_ty_own. iExists ly.
+    iSplitR. { destruct Hcompat as [<- | (ly1 & Hst' & ->)]; first done.
+      simpl. iPureIntro. eapply syn_type_has_layout_make_untyped; last done.
+      by eapply syn_type_has_layout_inj. }
+    iR. iSplitR. { rewrite /ty_own_val/=//. }
+    iSplitL "Hlb"; first by iFrame.
+    iSplitR "Hl".
+    { iModIntro. destruct wl; last done. simpl. rewrite /num_cred. iFrame. iApply lc_succ; iFrame. }
+    iExists tt. iR. iModIntro. iExists _. iFrame.
+    rewrite uninit_own_spec. iExists ly.
+    apply syn_type_has_layout_ptr_inv in Halg as ->. iSplitR; last done.
+    iPureIntro. destruct Hcompat as [<- | (ly1 & Hst' & ->)]; first done.
+    specialize (syn_type_has_layout_ptr_inv _ Hst') as ->.
+    eapply syn_type_has_layout_make_untyped; done.
+  Qed.
+
+  Lemma ltype_uniq_extractable_deinit_mut F π l st {rt} (lt : ltype rt) r κ κm γ wl :
+    lftE ⊆ F →
+    ltype_uniq_extractable lt = Some κm →
+    syn_type_compat PtrSynType st →
+    (l ◁ₗ[π, Owned wl] #(r, γ) @ (MutLtype lt κ)) ={F}=∗
+    l ◁ₗ[π, Owned false] #() @ (◁ uninit st) ∗ MaybeInherit κm InheritGhost (place_rfn_interp_mut r γ).
+  Proof.
+    iIntros (? Hdeinit Hcompat).
+    iIntros "Hl".
+    rewrite ltype_own_mut_ref_unfold /mut_ltype_own.
+    iDestruct "Hl" as "(%ly & %Halg & %Hly & Hlb & Hcred & %γ' & %r' & %Heq & Hb)".
+    injection Heq as <- <-.
+    iMod (maybe_use_credit with "Hcred Hb") as "(Hcred & Hat & Hc)"; first done.
+    iDestruct "Hc" as "(%l' & Hl & Hb)".
+    iMod (ltype_own_extract_ghost_drop_uniq with "Hb") as "Hrfn"; [done.. | ].
+    iFrame.
+    rewrite ltype_own_ofty_unfold /lty_of_ty_own. iExists ly.
+    iSplitR. { destruct Hcompat as [<- | (ly1 & Hst' & ->)]; first done.
+      simpl. iPureIntro. eapply syn_type_has_layout_make_untyped; last done.
+      by eapply syn_type_has_layout_inj. }
+    iR. iSplitR. { rewrite /ty_own_val/=//. }
+    iSplitL "Hlb"; first done. iR.
+    iExists tt. iR. iModIntro. iExists _. iFrame.
+    rewrite uninit_own_spec. iExists ly.
+    apply syn_type_has_layout_ptr_inv in Halg as ->. iSplitR; last done.
+    iPureIntro. destruct Hcompat as [<- | (ly1 & Hst' & ->)]; first done.
+    specialize (syn_type_has_layout_ptr_inv _ Hst') as ->.
+    eapply syn_type_has_layout_make_untyped; done.
+  Qed.
+
+  (* TODO try to find a good way to unify with previous lemma *)
+  Lemma ltype_uniq_extractable_deinit_mut' F π l st {rt} (lt : ltype rt) r κ κm γ wl :
+    lftE ⊆ F →
+    ltype_uniq_extractable lt = Some κm →
+    syn_type_compat PtrSynType st →
+    £ (Nat.b2n wl) -∗
+    (l ◁ₗ[π, Owned wl] #(r, γ) @ (MutLtype lt κ)) ={F}=∗
+    l ◁ₗ[π, Owned wl] #() @ (◁ uninit st) ∗ MaybeInherit κm InheritGhost (place_rfn_interp_mut r γ).
+  Proof.
+    iIntros (? Hdeinit Hcompat).
+    iIntros "Hcred' Hl".
+    rewrite ltype_own_mut_ref_unfold /mut_ltype_own.
+    iDestruct "Hl" as "(%ly & %Halg & %Hly & Hlb & Hcred & %γ' & %r' & %Heq & Hb)".
+    injection Heq as <- <-.
+    iMod (maybe_use_credit with "Hcred Hb") as "(Hcred & Hat & Hc)"; first done.
+    iDestruct "Hc" as "(%l' & Hl & Hb)".
+    iMod (ltype_own_extract_ghost_drop_uniq with "Hb") as "Hrfn"; [done.. | ].
+    iFrame.
+    rewrite ltype_own_ofty_unfold /lty_of_ty_own. iExists ly.
+    iSplitR. { destruct Hcompat as [<- | (ly1 & Hst' & ->)]; first done.
+      simpl. iPureIntro. eapply syn_type_has_layout_make_untyped; last done.
+      by eapply syn_type_has_layout_inj. }
+    iR. iSplitR. { rewrite /ty_own_val/=//. }
+    iSplitL "Hlb"; first by iFrame.
+    iSplitR "Hl".
+    { iModIntro. destruct wl; last done. simpl. rewrite /num_cred. iFrame. iApply lc_succ; iFrame. }
+    iExists tt. iR. iModIntro. iExists _. iFrame.
+    rewrite uninit_own_spec. iExists ly.
+    apply syn_type_has_layout_ptr_inv in Halg as ->. iSplitR; last done.
+    iPureIntro. destruct Hcompat as [<- | (ly1 & Hst' & ->)]; first done.
+    specialize (syn_type_has_layout_ptr_inv _ Hst') as ->.
+    eapply syn_type_has_layout_make_untyped; done.
+  Qed.
+End deinit.
+
+Section extract.
+  Context `{!typeGS Σ}.
+
+  (* Extract an observation  *)
+  Lemma stratify_ltype_extract_ofty_mut π E L {rt} (ty : type rt) r κ γ l (wl : bool) (T : stratify_ltype_post_hook_cont_t) :
+    T L (place_rfn_interp_mut r γ) _ (◁ uninit PtrSynType)%I (#())
+    ⊢ stratify_ltype_post_hook π E L (StratifyExtractOp κ) l (◁ (mut_ref κ ty)) (#(r, γ)) (Owned wl) T.
+  Proof.
+    iIntros "HT".
+    iIntros (????) "#CTX #HE HL Hl".
+    rewrite ltype_own_ofty_unfold /lty_of_ty_own.
+    iExists _, _, _, _, _. iFrame.
+    iDestruct "Hl" as "(%ly & %Hst & %Hly & Hsc & Hlb & Hcreds & %r' & <- & Hb)".
+    iMod (maybe_use_credit with "Hcreds Hb") as "(Hcreds & Hat & Hb)"; first done.
+    iDestruct "Hb" as "(%v & Hl & Hb)".
+    rewrite /ty_own_val/=.
+    iDestruct "Hb" as "(% & % & -> & ? & ? & ? & ? & Hb & Hcred' & ?)".
+    iFrame.
+    iSplitR. { simp_ltypes. done. }
+    rewrite ltype_own_ofty_unfold /lty_of_ty_own.
+    iExists _. simpl. iFrame. iR. iR.
+    iSplitL "Hcred'". { destruct wl; last done. by iFrame. }
+    iExists _. iR. iModIntro. iModIntro. iModIntro.
+    rewrite uninit_own_spec. iExists _. iR.
+    iPureIntro. eapply syn_type_has_layout_ptr_inv in Hst. subst.
+    done.
+  Qed.
+  Global Instance stratify_ltype_extract_ofty_mut_inst π E L {rt} (ty : type rt) r κ γ l (wl : bool) :
+    StratifyLtypePostHook π E L (StratifyExtractOp κ) l (◁ (mut_ref κ ty))%I (#(r, γ)) (Owned wl) | 20 :=
+    λ T, i2p (stratify_ltype_extract_ofty_mut π E L ty r κ γ l wl T).
+
+  (* Extract an observation from the ltype *)
+  Lemma stratify_ltype_extract_mutltype π E L {rt} (lt : ltype rt) r κ γ l (wl : bool) (T : stratify_ltype_post_hook_cont_t) :
+    match ltype_uniq_extractable lt with
+    | None =>
+        T L True%I _ (MutLtype lt κ) (#(r, γ))
+    | Some κm =>
+        prove_with_subtype E L false ProveDirect (£ (Nat.b2n wl)) (λ L' κs R,
+          (R -∗ T L' (MaybeInherit κm InheritGhost (place_rfn_interp_mut_extracted r γ)) _ (◁ uninit PtrSynType)%I (#())))
+    end
+    ⊢ stratify_ltype_post_hook π E L (StratifyExtractOp κ) l (MutLtype lt κ) (#(r, γ)) (Owned wl) T.
+  Proof.
+    iIntros "HT".
+    iIntros (????) "#CTX #HE HL Hl".
+    destruct (ltype_uniq_extractable lt) as [ κm | ] eqn:Hextract; first last.
+    { iExists L, True%I, _, _, _. iFrame. done. }
+    iMod ("HT" with "[//] [//] [//] CTX HE HL") as "(%L' & %κs & %R & >(Hcred & HR)& HL & HT)".
+    iMod (ltype_uniq_extractable_deinit_mut' with "Hcred Hl") as "(Hl & Hrfn)"; [done.. | | ].
+    { left. done. }
+    iSpecialize ("HT" with "HR").
+    iPoseProof (MaybeInherit_update (place_rfn_interp_mut_extracted r γ) with "[] Hrfn") as "Ha".
+    { iIntros (?) "Ha". iMod (place_rfn_interp_mut_extract with "Ha") as "?". done. }
+    iExists _, _, _, _, _. iFrame.
+    iFrame. simp_ltypes. done.
+  Qed.
+  Global Instance stratify_ltype_extract_mutltype_inst π E L {rt} (lt : ltype rt) r κ γ l (wl : bool) :
+    StratifyLtypePostHook π E L (StratifyExtractOp κ) l (MutLtype lt κ) (#(r, γ)) (Owned wl) :=
+    λ T, i2p (stratify_ltype_extract_mutltype π E L lt r κ γ l wl T).
+End extract.
+
+Section rule.
+  Context `{!typeGS Σ}.
+
+  Lemma owned_subltype_step_mutltype_uninit π E L {rt} (lt : ltype rt) r γ st κ l T :
+    owned_subltype_step π E L l #(r, γ) #() (MutLtype lt κ) (◁ uninit st) T :-
+    return match ltype_uniq_extractable lt with
+    | None => False
+    | Some κm =>
+        [{ exhale (⌜syn_type_compat PtrSynType st⌝);
+        return T L (MaybeInherit κm InheritGhost (place_rfn_interp_mut_extracted r γ)) }]
+    end.
+  Proof.
+    iIntros "HT".
+    iIntros (??) "CTX HE HL Hl". simp_ltypes; simpl.
+    destruct (ltype_uniq_extractable lt) eqn:Hextract; last done.
+    iDestruct "HT" as "(%Hstcomp & HT)".
+    iExists _, _. iFrame.
+    iMod (ltype_uniq_extractable_deinit_mut with "Hl") as "(Hl & Hf)"; [done.. | ].
+    iPoseProof (MaybeInherit_update (place_rfn_interp_mut_extracted r γ) with "[] Hf") as "Hf".
+    { iIntros (?) "Hrfn". iMod (place_rfn_interp_mut_extract with "Hrfn") as "?". done. }
+    iModIntro. iSplitL. { iApply logical_step_intro. iFrame. }
+    iPureIntro. iIntros (ly1 ly2 Halg1 Halg2).
+    specialize (syn_type_compat_layout_trans _ _ _ Hstcomp Halg2) as ?.
+    f_equiv. by eapply syn_type_has_layout_inj.
+  Qed.
+  Definition owned_subltype_step_mutltype_uninit_inst := [instance owned_subltype_step_mutltype_uninit].
+  Global Existing Instance owned_subltype_step_mutltype_uninit_inst | 20.
+End rule.
