theories/rust_typing/mut_ref/mut_ref.v
@@ -1,4 +1,4 @@
 From refinedrust Require Export base type ltypes.
-From refinedrust.mut_ref Require Export def borrow place resolve_ghost stratify subltype subtype subtype_instances unfold.
+From refinedrust.mut_ref Require Export def borrow place resolve_ghost stratify subltype subtype subtype_instances unfold deinit.
 
 
