theories/rust_typing/mut_ref/stratify.v
@@ -1,70 +1,9 @@
 From refinedrust Require Export base type ltypes.
 From refinedrust Require Import programs.
-From refinedrust.mut_ref Require Import def subltype unfold. 
+From refinedrust.mut_ref Require Import def subltype unfold.
 From refinedrust Require Import options.
 
 (** ** Stratification rules for mutable references *)
-Section extract.
-  Context `{!typeGS Σ}.
-
-  (* Extract an observation  *)
-  Lemma stratify_ltype_extract_ofty_mut π E L {rt} (ty : type rt) r κ γ l (wl : bool) (T : stratify_ltype_post_hook_cont_t) :
-    T L (place_rfn_interp_mut r γ) _ (◁ uninit PtrSynType)%I (#())
-    ⊢ stratify_ltype_post_hook π E L (StratifyExtractOp κ) l (◁ (mut_ref κ ty)) (#(r, γ)) (Owned wl) T.
-  Proof.
-    iIntros "HT".
-    iIntros (????) "#CTX #HE HL Hl".
-    rewrite ltype_own_ofty_unfold /lty_of_ty_own.
-    iExists _, _, _, _, _. iFrame.
-    iDestruct "Hl" as "(%ly & %Hst & %Hly & Hsc & Hlb & Hcreds & %r' & <- & Hb)".
-    iMod (maybe_use_credit with "Hcreds Hb") as "(Hcreds & Hat & Hb)"; first done.
-    iDestruct "Hb" as "(%v & Hl & Hb)".
-    rewrite /ty_own_val/=.
-    iDestruct "Hb" as "(% & % & -> & ? & ? & ? & ? & Hb & Hcred' & ?)".
-    iFrame.
-    iSplitR. { simp_ltypes. done. }
-    rewrite ltype_own_ofty_unfold /lty_of_ty_own.
-    iExists _. simpl. iFrame. iR. iR.
-    iSplitL "Hcred'". { destruct wl; last done. by iFrame. }
-    iExists _. iR. iModIntro. iModIntro. iModIntro.
-    rewrite uninit_own_spec. iExists _. iR.
-    iPureIntro. eapply syn_type_has_layout_ptr_inv in Hst. subst.
-    done.
-  Qed.
-  Global Instance stratify_ltype_extract_ofty_mut_inst π E L {rt} (ty : type rt) r κ γ l (wl : bool) :
-    StratifyLtypePostHook π E L (StratifyExtractOp κ) l (◁ (mut_ref κ ty))%I (#(r, γ)) (Owned wl) | 20 :=
-    λ T, i2p (stratify_ltype_extract_ofty_mut π E L ty r κ γ l wl T).
-
-  (* Extract an observation from the ltype *)
-  Lemma stratify_ltype_extract_mutltype π E L {rt} (lt : ltype rt) r κ γ l (wl : bool) (T : stratify_ltype_post_hook_cont_t) :
-    match ltype_uniq_extractable lt with
-    | None =>
-        T L True%I _ (MutLtype lt κ) (#(r, γ))
-    | Some κm =>
-        prove_with_subtype E L false ProveDirect (£ (Nat.b2n wl)) (λ L' κs R,
-          (R -∗ T L' (MaybeInherit κm InheritGhost (place_rfn_interp_mut_extracted r γ)) _ (◁ uninit PtrSynType)%I (#())))
-    end
-    ⊢ stratify_ltype_post_hook π E L (StratifyExtractOp κ) l (MutLtype lt κ) (#(r, γ)) (Owned wl) T.
-  Proof.
-    iIntros "HT".
-    iIntros (????) "#CTX #HE HL Hl".
-    destruct (ltype_uniq_extractable lt) as [ κm | ] eqn:Hextract; first last.
-    { iExists L, True%I, _, _, _. iFrame. done. }
-    iMod ("HT" with "[//] [//] [//] CTX HE HL") as "(%L' & %κs & %R & >(Hcred & HR)& HL & HT)".
-    iMod (ltype_uniq_extractable_deinit_mut' with "Hcred Hl") as "(Hl & Hrfn)"; [done.. | | ].
-    { left. done. }
-    iSpecialize ("HT" with "HR").
-    iPoseProof (MaybeInherit_update (place_rfn_interp_mut_extracted r γ) with "[] Hrfn") as "Ha".
-    { iIntros (?) "Ha". iMod (place_rfn_interp_mut_extract with "Ha") as "?". done. }
-    iExists _, _, _, _, _. iFrame.
-    iFrame. simp_ltypes. done.
-  Qed.
-  Global Instance stratify_ltype_extract_mutltype_inst π E L {rt} (lt : ltype rt) r κ γ l (wl : bool) :
-    StratifyLtypePostHook π E L (StratifyExtractOp κ) l (MutLtype lt κ) (#(r, γ)) (Owned wl) :=
-    λ T, i2p (stratify_ltype_extract_mutltype π E L lt r κ γ l wl T).
-
-End extract.
-
 Section stratify.
   Context `{!typeGS Σ}.
 
