theories/rust_typing/shr_ref/shr_ref.v
@@ -1,4 +1,4 @@
 From refinedrust Require Export base type ltypes.
-From refinedrust.shr_ref Require Export def borrow place stratify subltype subtype subtype_instances unfold.
+From refinedrust.shr_ref Require Export def borrow place stratify subltype subtype subtype_instances unfold deinit.
 
 
