theories/rust_typing/struct/deinit.v
@@ -1,0 +1,85 @@
+From refinedrust Require Export base type ltypes.
+From refinedrust Require Import ltype_rules.
+From refinedrust Require Import programs struct.subltype.
+From refinedrust Require Import options.
+
+(** ** Lemmas about deinitializing *)
+
+Section deinit.
+  Context `{!typeGS Σ}.
+
+
+  (* TODO *)
+  Lemma ltype_deinit_struct F π {rts} (lts : hlist ltype rts) (sls : struct_layout_spec) rs st l wl :
+    lftE ⊆ F →
+    syn_type_compat sls st →
+    (l ◁ₗ[π, Owned wl] rs @ (StructLtype lts sls)) ={F}=∗
+    l ◁ₗ[π, Owned false] #() @ (◁ uninit st).
+  Proof.
+    iIntros (? Hstcomp) "Hl".
+    rewrite ltype_own_struct_unfold /struct_ltype_own.
+    (* this doesn't hold because we might have an alias. *)
+
+    (*
+    iDestruct "Hl" as "(%ly & %Halg & % & Hlb & Hcreds & %r' & ? & Hb)".
+    iMod (maybe_use_credit with "Hcreds Hb") as "(? & ? & %l' & Hl & Hb)"; first done.
+    rewrite ltype_own_ofty_unfold /lty_of_ty_own.
+    iModIntro. iExists ly. simpl. iSplitR.
+    { destruct Hstcomp as [<- | (ly1 & Hst' & ->)]; first done.
+      simpl. iPureIntro. eapply syn_type_has_layout_make_untyped; last done.
+      by eapply syn_type_has_layout_inj. }
+    iR. iR.
+    iSplitL "Hlb"; first by iFrame. iR.
+    iExists tt. iR.
+    iModIntro. iExists l'. iFrame. rewrite uninit_own_spec. iExists ly.
+    apply syn_type_has_layout_ptr_inv in Halg as ->. iSplitR; last done.
+    iPureIntro. destruct Hstcomp as [<- | (ly1 & Hst' & ->)]; first done.
+    specialize (syn_type_has_layout_ptr_inv _ Hst') as ->.
+    eapply syn_type_has_layout_make_untyped; done.
+  Qed.
+     *)
+  Abort.
+
+End deinit.
+
+Section rules.
+  Context `{!typeGS Σ}.
+
+  (* We iterate over all the fields to deinitialize them first, and then deinitialize the struct itself *)
+  Lemma owned_subltype_step_struct_uninit π E L l {rts} (lts : hlist ltype rts) rs sls st T :
+    owned_subltype_step π E L l #rs #() (StructLtype lts sls) (◁ uninit st) T :-
+    exhale (⌜st = sls⌝);
+    L2, R2 ← iterate: zip (hpzipl rts lts rs) sls.(sls_fields) with L, True%I {{ '((existT rt (lt, r)), (field, stf)) T L2 R2,
+      return owned_subltype_step π E L2 (l atst{sls}ₗ field) r #() lt (◁ uninit stf) (λ L3 R3,
+        T L3 (R2 ∗ R3))
+      }};
+    return T L2 R2.
+  Proof.
+    iIntros "(-> & Hit)".
+    iIntros (??) "#CTX #HE HL Hl".
+
+    rewrite ltype_own_struct_unfold/struct_ltype_own/=.
+    iDestruct "Hl" as "(%sl & %Halg & %Hlen & %Hly & Hlb & _ & %rs' & -> & Hl)".
+    iMod (fupd_mask_mono with "Hl") as "Hl"; first done.
+
+    iPoseProof (struct_ltype_focus_components with "Hl") as "(Hl & Hclose_l)"; [done.. | ].
+    Search li.iterate "elim".
+    (* invariant: ownership of the first n uninit segments.
+        ownership for the rest
+    *)
+
+    (*
+    set (INV := λ (i : nat) (L2 : llctx) (R2 : iProp Σ),
+      llctx_interp L2 ∗
+
+      logical_step F ( ∗ R2)).
+     *)
+
+    (*Search iterate_elim2*)
+
+  Admitted.
+  Definition owned_subltype_step_struct_uninit_inst := [instance owned_subltype_step_struct_uninit].
+  Global Existing Instance owned_subltype_step_struct_uninit_inst | 20.
+
+  (* TODO: extractop *)
+End rules.
