theories/rust_typing/struct/struct.v
@@ -1,2 +1,2 @@
 From refinedrust Require Export type ltypes.
-From refinedrust.struct Require Export def init place resolve_ghost stratify subltype subtype subtype_instances unfold.
+From refinedrust.struct Require Export def init place resolve_ghost stratify subltype subtype subtype_instances unfold deinit.
